experiment/Experiment.Steel.Repr.LV_to_M.fst
@@ -1,6 +1,97 @@
 module Experiment.Steel.Repr.LV_to_M
 
+module L      = FStar.List.Pure
+module Fl     = Learn.FList
+module Veq    = Experiment.Steel.VEquiv
+module Perm   = Learn.Permutation
+module TLogic = Learn.Tactics.Logic
+
 open FStar.Tactics
+
+#push-options "--ifuel 0 --fuel 0"
+let extract_eij_framed_equiv
+      (env : vprop_list) (pre : M.pre_t) (csm_f : eq_injection_l pre env)
+      (sl : sl_f env)
+  : Lemma (extract_vars (eij_framed_equiv env pre csm_f) sl
+        == append_vars (eij_sl (L.index csm_f) sl) (filter_sl (mask_not (eij_trg_mask csm_f)) sl))
+  =
+    Ll.pat_append ();
+    let m = eij_trg_mask csm_f in
+    let flt1 = filter_mask (mask_not m) env in
+    let l1 = L.(filter_mask m env @ flt1) in
+    let l2 = L.(pre @ flt1) in
+    let f0 : vequiv_perm env l1 = mask_pequiv_append m env in
+    let f1 : vequiv_perm l1  l2 = Perm.(pequiv_append (eij_equiv csm_f) (pequiv_refl flt1)) in
+    calc (==) {
+      extract_vars (eij_framed_equiv env pre csm_f) sl <: sl_f l2;
+    == { }
+      extract_vars Perm.(pequiv_trans f0 f1) sl;
+    == { Fl.apply_pequiv_trans (vequiv_perm_sl f0) (vequiv_perm_sl f1) sl }
+      extract_vars f1 (extract_vars f0 sl);
+    == { filter_mask_fl_perm_append m (vprop_list_sels_t env) sl }
+      extract_vars f1 (Fl.append (filter_sl m sl) (filter_sl (mask_not m) sl));
+    == { Fl.apply_pequiv_append (vequiv_perm_sl (eij_equiv csm_f)) (vequiv_perm_sl (Perm.pequiv_refl flt1))
+                                (filter_sl m sl) (filter_sl (mask_not m) sl) }
+      Fl.append (extract_vars (eij_equiv csm_f) (filter_sl m sl))
+                (extract_vars (Perm.pequiv_refl flt1) (filter_sl (mask_not m) sl));
+    == { }
+      Fl.append (extract_vars (eij_equiv csm_f) (filter_sl m sl)) (filter_sl (mask_not m) sl);
+    == { extract_eij_equiv csm_f sl }
+      Fl.append #(vprop_list_sels_t pre) (eij_sl (L.index csm_f) sl) (filter_sl (mask_not m) sl);
+    }
+
+let extract_sub_prd_framed_equiv
+      (env : vprop_list) 
+      (csm0 : csm_t env) (prd0 : vprop_list)
+      (csm1 : csm_t (filter_mask (mask_not csm0) env)) (prd1 : vprop_list)
+      (veq  : vequiv_perm (sub_prd env csm0 prd0 csm1) prd1)
+      (sl0 : sl_f prd0) (sl1 : sl_f (filter_mask (mask_not csm0) env))
+  : Lemma (filter_bind_csm env csm0 csm1;
+       extract_vars (sub_prd_framed_equiv env csm0 prd0 csm1 prd1 veq) (append_vars sl0 sl1)
+    == append_vars (extract_vars veq (append_vars sl0 (filter_sl csm1 sl1)))
+                   (filter_sl (mask_not csm1) sl1))
+  =
+    Ll.pat_append ();
+    filter_bind_csm env csm0 csm1;
+    let env1 = filter_mask (mask_not csm0) env  in
+    let flt1 = filter_mask csm1 env1            in
+    let flt2 = filter_mask (mask_not csm1) env1 in
+    L.append_assoc prd0 flt1 flt2;
+
+    let f0  : vequiv_perm L.(prd0 @ flt1) prd1 = U.cast _ veq    in
+    let f0' : vequiv_perm L.(prd0 @ flt1 @ flt2) L.(prd1 @ flt2)
+      = U.cast _ (Perm.pequiv_append f0 (Perm.pequiv_refl flt2)) in
+    let f1  : vequiv_perm env1 L.(flt1 @ flt2)
+       = mask_pequiv_append csm1 env1                            in
+    let f1' : vequiv_perm L.(prd0 @ env1) L.(prd0 @ flt1 @ flt2)
+      = Perm.pequiv_append (Perm.pequiv_refl prd0) f1            in
+    let sls0 : sl_f L.(prd0 @ env1) = Fl.append sl0 sl1          in
+    let sl_flt1 : sl_f flt1 = filter_sl csm1 sl1                 in
+    let sl_flt2 : sl_f flt2 = filter_sl (mask_not csm1) sl1      in
+
+    calc (==) {
+      extract_vars (sub_prd_framed_equiv env csm0 prd0 csm1 prd1 veq) (append_vars sl0 sl1)
+        <: sl_f L.(prd1 @ flt2);
+    == { }
+      extract_vars (Perm.pequiv_trans f1' f0') sls0;
+    == { Fl.apply_pequiv_trans (vequiv_perm_sl f1') (vequiv_perm_sl f0') sls0 }
+      extract_vars f0' (extract_vars f1' sls0);
+    == { Fl.apply_pequiv_append (vequiv_perm_sl (Perm.pequiv_refl prd0))
+                                (vequiv_perm_sl f1)
+                                sl0 sl1 }
+      extract_vars f0' (append_vars sl0 (extract_vars f1 sl1));
+    == { filter_mask_fl_perm_append csm1 (vprop_list_sels_t env1) sl1 }
+      extract_vars f0' (append_vars sl0 (append_vars sl_flt1 sl_flt2));
+    == { Fl.append_assoc sl0 sl_flt1 sl_flt2 }
+      extract_vars f0' (append_vars (append_vars sl0 sl_flt1) sl_flt2);
+    == { Fl.apply_pequiv_append (vequiv_perm_sl f0)
+                                (vequiv_perm_sl (Perm.pequiv_refl flt2))
+                                (append_vars sl0 sl_flt1) sl_flt2 }
+      append_vars (extract_vars veq (append_vars sl0 sl_flt1)) sl_flt2;
+    }
+
+#pop-options
+
 
 let bind_g_csm'_res_env_f
       (env : vprop_list) (b : Type)
@@ -14,3 +105,327 @@ let bind_g_csm'_res_env_f
         (res_env_f env (bind_csm env f_csm g_csm) g_prd)
         (_ by (trefl ())) (_ by (trefl ()))
         (fun (x : b) -> filter_bind_g_csm' env f_csm f_prd g_csm)
+
+
+(*** Soundness *)
+
+#push-options "--ifuel 0 --fuel 0"
+
+let sound_repr_M_of_LV
+      (#env : vprop_list) (#a : Type u#a) (#t : M.prog_tree a)
+      (#csm : csm_t env) (#prd : prd_t a)
+      (lc : lin_cond env t csm prd {lcsub_at_leaves lc})
+  : prop
+  = sound_M_of_LV lc (repr_M_of_LV lc)
+
+let intro_sound_M_of_LV
+      (#env : vprop_list) (#a : Type u#a) (#t : M.prog_tree a)
+      (#csm : csm_t env) (#prd : prd_t a)
+      (lc : lin_cond env t csm prd) (mc : lc_to_M lc)
+      (pf_req : (sl0 : sl_f env) ->
+                squash (M.tree_req t mc sl0 <==> tree_req lc sl0))
+      (pf_ens : (sl0 : sl_f env) -> (res : a) -> (sl1 : sl_f (prd res)) ->
+                (sl_rem : sl_f (filter_mask (mask_not csm) env)) ->
+                squash (M.tree_ens t mc sl0 res (res_env_app sl1 sl_rem) <==>
+                        (tree_ens lc sl0 res sl1 /\ sl_rem == filter_sl (mask_not csm) sl0)))
+  : squash (sound_M_of_LV lc mc)
+  =
+    introduce forall (sl0 : sl_f env) . M.tree_req t mc sl0 <==> tree_req lc sl0
+      with pf_req sl0;
+    introduce forall (sl0 : sl_f env) (res : a) (sl1 : sl_f (prd res))
+                (sl_rem : sl_f (filter_mask (mask_not csm) env)) .
+                M.tree_ens t mc sl0 res (res_env_app sl1 sl_rem) <==>
+                (tree_ens lc sl0 res sl1 /\ sl_rem == filter_sl (mask_not csm) sl0)
+      with pf_ens sl0 res sl1 sl_rem
+
+let sound_M_of_LV_req
+      #env #a #t #csm #prd
+      (#lc : lin_cond env #a t csm prd) (#mc : lc_to_M lc)
+      (pf : squash (sound_M_of_LV lc mc))
+      (sl0 : sl_f env) 
+  : squash (M.tree_req t mc sl0 <==> tree_req lc sl0)
+  = ()
+
+let sound_M_of_LV_ens
+      #env #a #t #csm #prd
+      (#lc : lin_cond env #a t csm prd) (#mc : lc_to_M lc)
+      (pf : squash (sound_M_of_LV lc mc))
+      (sl0 : sl_f env) (res : a) (sl1 : sl_f (prd res)) (sl_rem : sl_f (filter_mask (mask_not csm) env))
+  : squash (M.tree_ens t mc sl0 res (res_env_app sl1 sl_rem) <==>
+             (tree_ens lc sl0 res sl1 /\ sl_rem == filter_sl (mask_not csm) sl0))
+  = ()
+
+
+let vequiv_of_perm_sel_eq_list
+      (#pre #post : vprop_list) (f : vequiv_perm pre post)
+      (sl0 : sl_f pre) (sl1 : sl_f post)
+  : squash Veq.(veq_sel_eq (veq_eq_sl (veq_of_list (veq_to_list (vequiv_of_perm_eq f)))) sl0 sl1
+                <==> sl1 == extract_vars f sl0)
+  = Veq.vequiv_of_perm_sel_eq f sl0 sl1
+
+let rew_append_var_inj (#t0 #t1 : vprop_list) (x0 x1 : sl_f t0) (y0 y1 : sl_f t1)
+  : squash ((append_vars x0 y0 == append_vars x1 y1) <==> (x0 == x1 /\ y0 == y1))
+  = Fl.append_splitAt_ty _ _ x0 y0; Fl.append_splitAt_ty _ _ x1 y1
+
+let rew_append_var_inj'
+    #tx0 (x0 : sl_f tx0) #tx1 (x1 : sl_f tx1)
+    #ty0 (y0 : sl_f ty0) #ty1 (y1 : sl_f ty1)
+    #teq (_ : squash (tx0 == tx1 /\ ty0 == ty1 /\ teq == L.(tx0 @ ty0)))
+  : squash (eq2 #(sl_f teq) (append_vars #tx0 #ty0 x0 y0) (append_vars #tx1 #ty1 x1 y1)
+        <==> (x0 == x1 /\ y0 == y1))
+  = rew_append_var_inj x0 x1 y0 y1
+
+let rew_forall_sl_f_app (v0 v1 : vprop_list) (p0 : sl_f L.(v0 @ v1) -> Type) (p1 : Type)
+    (_ : squash ((forall (sl0 : sl_f v0) (sl1 : sl_f v1) . p0 (append_vars sl0 sl1)) <==> p1))
+  : squash ((forall (sl : sl_f L.(v0 @ v1)) . p0 sl) <==> p1)
+  =
+    introduce (forall (sl0 : sl_f v0) (sl1 : sl_f v1) . p0 (append_vars sl0 sl1)) ==>
+              (forall (sl : sl_f L.(v0 @ v1)) . p0 sl)
+      with _ . introduce forall sl . _
+      with (let sl0, sl1 = split_vars v0 v1 sl in
+            Ll.pat_append ();
+            FStar.Classical.forall_intro (Fl.splitAt_ty_append (vprop_list_sels_t v0) (vprop_list_sels_t v1));
+            assert (sl == append_vars sl0 sl1);
+            eliminate forall (sl0 : sl_f v0) (sl1 : sl_f v1) . p0 (append_vars sl0 sl1) with sl0 sl1);
+    introduce (forall (sl : sl_f L.(v0 @ v1)) . p0 sl) ==>
+              (forall (sl0 : sl_f v0) (sl1 : sl_f v1) . p0 (append_vars sl0 sl1))
+      with _ . introduce forall sl0 sl1 . _
+      with eliminate forall (sl : sl_f L.(v0 @ v1)) . p0 sl with (append_vars sl0 sl1)
+
+let rew_exists_sl_f_app (v0 v1 : vprop_list) (p0 : sl_f L.(v0 @ v1) -> Type) (p1 : Type)
+    (_ : squash ((exists (sl0 : sl_f v0) (sl1 : sl_f v1) . p0 (append_vars sl0 sl1)) <==> p1))
+  : squash ((exists (sl : sl_f L.(v0 @ v1)) . p0 sl) <==> p1)
+  =
+    introduce (exists (sl0 : sl_f v0) (sl1 : sl_f v1) . p0 (append_vars sl0 sl1)) ==>
+              (exists (sl : sl_f L.(v0 @ v1)) . p0 sl)
+      with _ . eliminate exists (sl0 : sl_f v0) (sl1 : sl_f v1) . p0 (append_vars sl0 sl1)
+      returns _
+      with _ . introduce exists (sl : sl_f L.(v0 @ v1)) . p0 sl
+        with (append_vars sl0 sl1) and ();
+    introduce (exists (sl : sl_f L.(v0 @ v1)) . p0 sl) ==>
+              (exists (sl0 : sl_f v0) (sl1 : sl_f v1) . p0 (append_vars sl0 sl1))
+      with _ . eliminate exists (sl : sl_f L.(v0 @ v1)) . p0 sl
+      returns _
+      with _ . (
+         let sl0, sl1 = split_vars v0 v1 sl in
+         Ll.pat_append ();
+         FStar.Classical.forall_intro (Fl.splitAt_ty_append (vprop_list_sels_t v0) (vprop_list_sels_t v1));
+         assert (sl == append_vars sl0 sl1);
+         introduce exists (sl0 : sl_f v0) (sl1 : sl_f v1) . p0 (append_vars sl0 sl1)
+           with sl0 sl1 and ())
+
+#pop-options
+
+let vequiv_refl_sel_eq
+      (#v: vprop_list) (sl0 : sl_f v) (sl1 : sl_f v)
+  : squash Veq.(veq_sel_eq (veq_eq_sl (veq_of_list (vequiv_refl_eq v))) sl0 sl1 <==> sl1 == sl0)
+  = introduce _ /\  _
+       with introduce _ ==> _ with _ .
+            Fl.flist_extensionality sl1 sl0 (fun i -> ())
+        and ()
+
+
+let rew_iff_LV2M () : Tac unit =
+  TLogic.rew_iff (fun r -> first [
+    (fun () -> apply (`vequiv_refl_sel_eq));
+    (fun () -> apply (`vequiv_of_perm_sel_eq_list));
+    (fun () -> apply (`rew_append_var_inj));
+    (fun () -> apply (`rew_append_var_inj'); later ());
+    (fun () -> apply (`rew_forall_sl_f_app); r ());
+    (fun () -> apply (`rew_exists_sl_f_app); r ())
+  ])
+
+let norm_sound_LV2M () : Tac unit =
+  norm [delta_only [`%repr_M_of_LV; `%repr_M_of_LV__tcs; `%repr_M_of_LV__tcs_sub;
+                    `%M.tree_req; `%M.spec_req; `%M.return_req; `%M.bind_req;
+                    `%M.tree_ens; `%M.spec_ens; `%M.return_ens; `%M.bind_ens;
+                    `%Veq.vequiv_of_perm; `%Veq.vequiv_refl;
+                    `%Veq.Mkvequiv?.veq_req; `%Veq.Mkvequiv?.veq_ens; `%Veq.Mkvequiv?.veq_eq; `%Veq.veq_ens1;
+                    `%tree_req; `%tree_ens;
+                    `%res_env_app; `%res_env_f; `%res_env];
+        delta_attr [`%Learn.Tactics.Util.__tac_helper__];
+        iota; zeta]
+
+let tac_sound_LV2M () : Tac unit =
+  norm_sound_LV2M ();
+  apply (`TLogic.rew_iff_left); rew_iff_LV2M (); norm [simplify];
+  l_to_r [`extract_eij_framed_equiv];
+  apply (`TLogic.rew_iff_left); rew_iff_LV2M (); norm []
+
+
+#push-options "--ifuel 0 --fuel 1"
+
+let sound_repr_M_of_LV__LCspec
+      (env : vprop_list)
+      (a : Type u#a) (pre : M.pre_t) (post : M.post_t a)
+      (req : M.req_t pre) (ens : M.ens_t pre a post)
+      (csm_f : eq_injection_l pre env)
+  : squash (sound_repr_M_of_LV (LCspec env #a #pre #post #req #ens csm_f))
+  =
+    intro_sound_M_of_LV _ _
+      (fun sl0 ->
+        let sl0_0 = eij_sl #pre #env (L.index csm_f) sl0          in
+        let sl0_1 = filter_sl (mask_not (eij_trg_mask csm_f)) sl0 in
+        U.assert_by_tac (fun () ->
+              tac_sound_LV2M ();
+              // We rewrite [forall sl' . sl' = sl0_i ==> p sl'] into [p sl0_i]
+              TLogic.(
+                apply (`rew_iff_left); apply_raw (`rew_forall_eq (`@sl0_0));
+                  norm_sound_LV2M (); smt (); norm [simplify];
+                apply (`rew_iff_left); apply_raw (`rew_forall_eq (`@sl0_1));
+                  smt (); norm [simplify]
+              );
+              trivial ()))
+      (fun sl0 x sl1 sl_rem ->
+        _ by (tac_sound_LV2M ();
+              smt ()))
+
+let sound_repr_M_of_LV__LCret
+      (env : vprop_list)
+      (a : Type u#a) (x : a) (sl_hint : M.post_t a)
+      (prd : prd_t a) (csm_f : eq_injection_l (prd x) env)
+  : squash (sound_repr_M_of_LV (LCret env #a #x #sl_hint prd csm_f))
+  =
+    intro_sound_M_of_LV _ _
+      (fun sl0 -> ())
+      (fun sl0 x' sl1 sl_rem ->
+        _ by (tac_sound_LV2M ();
+                // [rew_append_var_inj'] generates an additional goal because the typing relies on [x' == x]
+                smt ();
+              smt ()))
+
+let sound_repr_M_of_LV__LCbind
+      (env : vprop_list)
+      (a : Type u#a) (b : Type u#a) (f : M.prog_tree a) (g : (a -> M.prog_tree b))
+      (f_csm : csm_t env) (f_prd : prd_t a)
+      (cf : lin_cond env f f_csm f_prd)
+      (g_csm : csm_t (filter_mask (mask_not f_csm) env)) (g_prd : prd_t b)
+      (cg : ((x : a) ->
+        lin_cond (res_env env f_csm (f_prd x)) (g x) (bind_g_csm' env f_csm (f_prd x) g_csm) g_prd))
+
+      (_ : squash (lcsub_at_leaves (LCbind env #a #b #f #g f_csm f_prd cf g_csm g_prd cg)))
+      (h_f : squash (sound_repr_M_of_LV cf))
+      (h_g : (x : a) -> squash (sound_repr_M_of_LV (cg x)))
+  : squash (sound_repr_M_of_LV (LCbind env #a #b #f #g f_csm f_prd cf g_csm g_prd cg))
+  =
+    introduce forall (x : a) .
+            res_env_f env (bind_csm env f_csm g_csm) g_prd
+         == res_env_f (res_env env f_csm (f_prd x)) (bind_g_csm' env f_csm (f_prd x) g_csm) g_prd
+      with bind_g_csm'_res_env_f env b f_csm (f_prd x) g_csm g_prd;
+    introduce forall (x : a) .
+            filter_mask (mask_not (bind_g_csm' env f_csm (f_prd x) g_csm)) (res_env env f_csm (f_prd x))
+         == filter_mask (mask_not (bind_csm env f_csm g_csm)) env
+      with filter_bind_g_csm' env f_csm (f_prd x) g_csm;
+    let h_g_req x sl0
+      : squash (M.tree_req (g x) #_ #(res_env_f env (bind_csm env f_csm g_csm) g_prd) (repr_M_of_LV (cg x)) sl0
+             <==> tree_req (cg x) sl0)
+      = sound_M_of_LV_req (h_g x) sl0
+    in let h_g_ens x (sl0 : sl_f (res_env env f_csm (f_prd x))) y sl1 sl_rem
+      : squash (M.tree_ens (g x)
+                  #_ #(res_env_f env (bind_csm env f_csm g_csm) g_prd) (repr_M_of_LV (cg x))
+                  sl0 y (res_env_app sl1 sl_rem)
+            <==> (tree_ens (cg x) sl0 y sl1 /\
+                sl_rem == filter_sl (mask_not (bind_g_csm' env f_csm (f_prd x) g_csm)) sl0))
+      = sound_M_of_LV_ens (h_g x) sl0 y sl1 sl_rem
+    in
+    intro_sound_M_of_LV _ _
+      (fun sl0 ->
+        _ by (norm_sound_LV2M ();
+              apply (`TLogic.rew_iff_left); rew_iff_LV2M (); norm [];
+              apply (`TLogic.rew_iff_left); TLogic.rew_iff (fun r -> first [
+                  (fun () -> apply (`sound_M_of_LV_req (`@h_f)));
+                  (fun () -> apply (`sound_M_of_LV_ens (`@h_f)));
+                  (fun () -> apply (``@h_g_req))
+                ]); norm [];
+              smt ()))
+      (fun sl0 y sl2 sl_rem ->
+        _ by (norm_sound_LV2M ();
+              apply (`TLogic.rew_iff_left); rew_iff_LV2M (); norm [];
+              apply (`TLogic.rew_iff_left); TLogic.rew_iff (fun r -> first [
+                  (fun () -> apply (`sound_M_of_LV_ens (`@h_f)));
+                  (fun () -> apply (``@h_g_ens))
+                ]); norm [];
+              l_to_r [`filter_sl_bind_g_csm'; `filter_sl_bind_csm];
+              smt ()
+              ))
+#pop-options
+
+// FIXME: without `--ide_id_info_off` the interactive mode takes a lot of time
+#push-options "--fuel 0 --ifuel 0 --ide_id_info_off"
+let sound_repr_M_of_LV__LCsub_LCspec
+      (env : vprop_list)
+      (a : Type u#a) (pre : M.pre_t) (post : M.post_t a)
+      (req : M.req_t pre) (ens : M.ens_t pre a post)
+      (csm_f : eq_injection_l pre env)
+      (csm1 : csm_t (filter_mask (mask_not (eij_trg_mask csm_f)) env))
+      (prd1 : prd_t a)
+      (prd_f1 : (x : a) -> Perm.pequiv_list (sub_prd env (eij_trg_mask csm_f) (post x) csm1) (prd1 x))
+  : (let lc = LCsub env (eij_trg_mask csm_f) post
+                     (LCspec env #a #pre #post #req #ens csm_f)
+                     csm1 prd1 prd_f1
+     in squash (lcsub_at_leaves lc /\ sound_repr_M_of_LV lc))
+  = introduce _ /\ _
+    with _ by (norm [delta_only [`%lcsub_at_leaves]; iota; zeta]; trivial ())
+    and intro_sound_M_of_LV _ _
+      (fun sl0 ->
+        let sl0_0 = eij_sl #pre #env (L.index csm_f) sl0          in
+        let sl0_1 = filter_sl (mask_not (eij_trg_mask csm_f)) sl0 in
+        U.assert_by_tac (fun () ->
+              tac_sound_LV2M ();
+              TLogic.(
+                apply (`rew_iff_left); apply_raw (`rew_forall_eq (`@sl0_0));
+                  norm_sound_LV2M (); smt (); norm [simplify];
+                apply (`rew_iff_left); apply_raw (`rew_forall_eq (`@sl0_1));
+                  smt (); norm [simplify]
+              );
+              trivial ()))
+      (fun sl0 x sl1 sl_rem ->
+        // A guard generated by [extract_sub_prd_framed_equiv]
+        let gd : squash (prd1 x == Perm.apply_perm_r (Perm.perm_f_of_list (prd_f1 x))
+                                                     (sub_prd env (eij_trg_mask csm_f) (post x) csm1))
+              = ()
+        in
+        _ by (with_policy Goal (fun () ->
+              norm_sound_LV2M ();
+              apply (`TLogic.rew_iff_left); rew_iff_LV2M (); norm [simplify];
+              l_to_r [`extract_eij_framed_equiv];
+              apply (`TLogic.rew_iff_left); rew_iff_LV2M (); norm [];
+              l_to_r [`extract_sub_prd_framed_equiv]);
+                later (); let _ = mintros () in exact (``@gd);
+              apply (`TLogic.rew_iff_left); rew_iff_LV2M ();
+                // additional goal generated by [rew_append_var_inj']
+                seq explode (fun () -> try trefl () with | _ -> ());
+                apply_lemma (`filter_bind_csm);
+              l_to_r [`filter_sl_bind_csm];
+              smt ()))
+#pop-options
+
+
+#push-options "--ifuel 1 --fuel 1"
+let rec repr_M_of_LV_sound
+      (#env : vprop_list) (#a : Type u#a) (#t : M.prog_tree a)
+      (#csm : csm_t env) (#prd : prd_t a)
+      (lc : lin_cond env t csm prd {lcsub_at_leaves lc})
+  : Lemma (ensures sound_M_of_LV lc (repr_M_of_LV lc)) (decreases lc)
+  = match lc with
+  | LCspec env #a #pre #post #req #ens csm_f ->
+      sound_repr_M_of_LV__LCspec env a pre post req ens csm_f
+  | LCret env #a #x #sl_hint prd csm_f ->
+      sound_repr_M_of_LV__LCret env a x sl_hint prd csm_f
+  | LCbind env #a #b #f #g f_csm f_prd cf g_csm g_prd cg ->
+      sound_repr_M_of_LV__LCbind env a b f g f_csm f_prd cf g_csm g_prd cg ()
+        (repr_M_of_LV_sound cf)
+        (fun (x : a) -> repr_M_of_LV_sound (cg x))
+  | LCsub env #a0 #f0 csm0 prd0 cf csm1 prd1 prd_f1 ->
+      let LCspec env #a #pre #post #req #ens csm_f = cf in
+      let csm0' = eij_trg_mask csm_f in
+      let prd0' = post in
+      let csm1' : csm_t (filter_mask (mask_not csm0) env) = csm1 in
+      U.arrow_ext #a (fun (x : a) -> Perm.pequiv_list (sub_prd env csm0' (prd0' x) csm1') (prd1 x))
+                     (fun (x : a) -> Perm.pequiv_list (sub_prd env csm0  (prd0  x) csm1 ) (prd1 x))
+                     (fun x -> ());
+      let prd_f1' : (x : a) -> Perm.pequiv_list (sub_prd env csm0' (prd0' x) csm1') (prd1 x)
+        = U.cast _ prd_f1 in
+      assert (lc == LCsub env csm0' prd0' (LCspec env #a #pre #post #req #ens csm_f) csm1' prd1 prd_f1');
+      sound_repr_M_of_LV__LCsub_LCspec env a pre post req ens csm_f csm1' prd1 prd_f1'
+#pop-options
