pure/Learn.List.Mask.fst
@@ -8,6 +8,12 @@ open FStar.List.Pure
 
 #push-options "--ifuel 1 --fuel 1"
 
+let rec mask_len_le (mask : list bool)
+  : Lemma (ensures mask_len mask <= length mask) (decreases mask)
+  = match mask with
+  | [] -> ()
+  | _ :: mask -> mask_len_le mask
+
 let rec mask_not_len (#n : nat) ($mask : vec n bool)
   : Lemma (ensures mask_len (mask_not mask) = n - mask_len mask) (decreases n)
           [SMTPat (mask_len (mask_not mask))]
@@ -104,6 +110,27 @@ let rec mask_comp_or_index
   | true  :: m0, m1 | false :: m0, _  :: m1 ->
       if i > 0 then mask_comp_or_index #(len-1) m0 m1 (i-1)
 
+let rec mask_comp_and_index
+      (#len : nat) (m0 : vec len bool) (m1 : vec (mask_len m0) bool) (i : Fin.fin len)
+  : Lemma (ensures   index (mask_comp_and m0 m1) i == (index m0 i && index m1 (mask_push m0 i)))
+          (decreases len)
+          [SMTPat (index (mask_comp_and m0 m1) i)]
+  = match m0, m1 with
+  | [], []  -> ()
+  | false  :: m0, m1 | true :: m0, _  :: m1 ->
+      if i > 0 then mask_comp_and_index #(len-1) m0 m1 (i-1)
+
+let rec mask_pull_comp_and
+      (#len : nat) (m0 : vec len bool) (m1 : vec (mask_len m0) bool) (i : Fin.fin (mask_len (mask_comp_and m0 m1)))
+  : Lemma (ensures   mask_pull (mask_comp_and m0 m1) i == mask_pull m0 (mask_pull m1 i))
+          (decreases len)
+  = match m0, m1 with
+  | false  :: m0, m1 | true :: m0, false  :: m1 ->
+      mask_pull_comp_and #(len-1) m0 m1 i
+  | true :: m0, true  :: m1 ->
+      if i > 0 then mask_pull_comp_and #(len-1) m0 m1 (i-1)
+
+
 let rec mask_comp_or_assoc #len m0 m1 m2
   : Lemma (ensures   mask_comp_or (mask_comp_or m0 m1) m2 == mask_comp_or m0 (mask_comp_or m1 m2))
           (decreases m0)
@@ -129,20 +156,79 @@ let rec filter_mask_and #a #len m0 m1 l
 
 #push-options "--z3rlimit 20"
 
-let rec filter_mask_perm_append_inv (#n : nat) (m : vec n bool)
+let rec mask_perm_append_inv (#n : nat) (m : vec n bool)
   : Lemma (ensures Perm.inv_f (mask_perm_append m) == mask_perm_append' m)
           (decreases n)
   = Perm.(match m with
   | [] -> ()
   | true :: m' ->
       let m' : vec (n-1) bool = m' in
-      filter_mask_perm_append_inv m'
+      mask_perm_append_inv m'
   | false :: m' ->
       let m' : vec (n-1) bool = m' in
-      filter_mask_perm_append_inv m';
+      mask_perm_append_inv m';
       let p0 = perm_cast n (perm_f_move_head (mask_len m') (mask_len (mask_not m'))) in
       let p1 = perm_cast n (perm_f_cons (mask_perm_append m')) in
       inv_f_comp p0 p1)
+
+#push-options "--ifuel 0 --fuel 1 --z3rlimit 40"
+let rec mask_perm_append'_index (#n : nat) (m : vec n bool) (i : Fin.fin n)
+  : Lemma (mask_perm_append' m i == (if index m i then mask_push m i else mask_len m + mask_push (mask_not m) i))
+  = match m with
+  | true :: m' ->
+      let m' : vec (n-1) bool = m' in
+      if i > 0 then begin
+        mask_perm_append'_index m' (i-1);
+        assert (index m i == index m' (i-1));
+        assert (mask_len m == mask_len m' + 1);
+        assert (mask_perm_append' m i == mask_perm_append' m' (i-1) + 1);
+        if index m i
+        then assert (mask_push m i == mask_push m' (i-1) + 1)
+        else assert (mask_push (mask_not m) i == mask_push (mask_not m') (i-1))
+      end
+  | false :: m' ->
+      let m  : vec   n   bool = false :: m' in
+      let m' : vec (n-1) bool = m'         in
+      assert (mask_len m == mask_len m');
+      if i > 0 then begin
+        mask_perm_append'_index m' (i-1);
+        assert (index m i == index m' (i-1));
+        assert (mask_perm_append' m i
+             == Perm.perm_f_move_to_head (mask_len m') (mask_len (mask_not m'))
+                                              (mask_perm_append' m' (i-1) + 1));
+        if index m i
+        then assert (mask_push m i == mask_push m' (i-1))
+        else begin
+          calc (==) {
+            mask_perm_append' m i;
+          == { }
+            Perm.perm_f_move_to_head (mask_len m') (mask_len (mask_not m'))
+                          (mask_len m' + mask_push (mask_not m') (i-1) + 1);
+          == { }
+            mask_len m' + mask_push (mask_not m') (i-1) + 1;
+          == { }
+            mask_len m + mask_push (mask_not m) i;
+          }
+        end
+      end
+#pop-options
+
+let mask_perm_append_index (#n : nat) (m : vec n bool) (i : Fin.fin n)
+  : Lemma (mask_perm_append m i =
+          (if i < mask_len m then mask_pull m i else mask_pull (mask_not m) (i - mask_len m)))
+  =
+    mask_len_le m;
+    let f (i : Fin.fin n) : Fin.fin n =
+      if i < mask_len m then mask_pull m i else mask_pull (mask_not m) (i - mask_len m)
+    in let f' (i : Fin.fin n) : Fin.fin n =
+      if index m i then mask_push m i else mask_len m + mask_push (mask_not m) i
+    in
+    let j = f i in
+    assert (f' j == i);
+    mask_perm_append'_index m j;
+    mask_perm_append_inv m;
+    Perm.pat_inv_f ()
+
 
 let tac_filter_mask_perm_append () : Tac unit =
   norm [delta_only [`%mask_perm_append]; zeta];
@@ -177,7 +263,7 @@ let filter_mask_perm_append' (#a : Type) (#n : nat) (m : vec n bool) (l : vec n 
   : Lemma (l == Perm.apply_perm_r (mask_perm_append' m) (filter_mask m l @ filter_mask (mask_not m) l))
   =
     filter_mask_perm_append m l;
-    filter_mask_perm_append_inv m;
+    mask_perm_append_inv m;
     Perm.apply_r_comp (mask_perm_append' m) (mask_perm_append m) l
 
 
@@ -186,6 +272,7 @@ let tac_filter_mask_or () : Tac unit =
   norm [iota];
   norm [delta_only [`%U.cast]; iota]
 
+#push-options "--z3rlimit 60"
 let rec filter_mask_or_append
       (#a : Type) (#len : nat) (m0 : vec len bool) (m1 : vec (mask_len (mask_not m0)) bool) (l : vec len a)
   : Lemma (ensures filter_mask m0 l @ filter_mask m1 (filter_mask (mask_not m0) l)
@@ -219,6 +306,7 @@ let rec filter_mask_or_append
   | false :: m0, false :: m1, x :: xs ->
       let m0 : vec (len-1) bool = m0 in
       filter_mask_or_append m0 m1 xs
+#pop-options
 
 (*
 [@@__mask__]
@@ -280,3 +368,69 @@ let rec filter_mask_dl_index (#len : nat) (mask : vec len bool) (ts : vec len Ty
       let t0 :: ts = ts in
       let xs = Dl.DCons?.xs xs in
       filter_mask_dl_index #(len-1) mask ts xs i
+
+#push-options "--ifuel 1 --fuel 1"
+let rec filter_mask_dl_append
+      (#n0 #n1 : nat) (m0 : vec n0 bool) (m1 : vec n1 bool)
+      (ts0 : vec n0 Type) (ts1 : vec n1 Type)
+      (xs0 : Dl.dlist ts0) (xs1 : Dl.dlist ts1)
+  : Lemma
+    (ensures (filter_mask_append m0 m1 ts0 ts1;
+        filter_mask_dl #(n0 + n1) (m0 @ m1) (ts0 @ ts1) (Dl.append xs0 xs1)
+     == Dl.append (filter_mask_dl m0 ts0 xs0) (filter_mask_dl m1 ts1 xs1)))
+    (decreases n0)
+  = filter_mask_append m0 m1 ts0 ts1;
+  match m0 with
+  | [] -> let Dl.DNil = xs0 in ()
+  | _ :: m0 -> let Dl.DCons _ _ ts0 xs0 = xs0 in
+             filter_mask_dl_append #(n0-1) m0 m1 ts0 ts1 xs0 xs1
+#pop-options
+
+#push-options "--ifuel 0 --fuel 0"
+let filter_mask_fl_perm_append (#n : nat) (m : vec n bool) (ts : vec n Type) (xs : Fl.flist ts)
+  : Lemma (Fl.apply_pequiv (mask_pequiv_append m ts) xs
+        == Fl.append (filter_mask_fl m ts xs) (filter_mask_fl (mask_not m) ts xs))
+  = Fl.flist_extensionality
+      (Fl.apply_pequiv (mask_pequiv_append m ts) xs)
+      (Fl.append (filter_mask_fl m ts xs) (filter_mask_fl (mask_not m) ts xs))
+      (fun i -> mask_perm_append_index m i)
+
+let filter_mask_fl_and
+      (#len : nat) (m0 : vec len bool) (m1 : vec (mask_len m0) bool) (ts : vec len Type)
+      (xs : Fl.flist ts)
+  : Lemma (filter_mask_and m0 m1 ts;
+           filter_mask_fl (mask_comp_and m0 m1) ts xs == filter_mask_fl m1 _ (filter_mask_fl m0 ts xs))
+  =
+    filter_mask_and m0 m1 ts;
+    Fl.flist_extensionality
+      (filter_mask_fl (mask_comp_and m0 m1) ts xs)
+      (filter_mask_fl m1 _ (filter_mask_fl m0 ts xs))
+      (fun j -> ())
+
+let filter_mask_fl_append
+      (#n0 #n1 : nat) (m0 : vec n0 bool) (m1 : vec n1 bool)
+      (ts0 : vec n0 Type) (ts1 : vec n1 Type)
+      (xs0 : Fl.flist ts0) (xs1 : Fl.flist ts1)
+  : Lemma (filter_mask_append m0 m1 ts0 ts1;
+        filter_mask_fl #(n0 + n1) (m0 @ m1) (ts0 @ ts1) (Fl.append xs0 xs1)
+     == Fl.append (filter_mask_fl m0 ts0 xs0) (filter_mask_fl m1 ts1 xs1))
+  =
+    let m : vec (n0+n1) bool = m0 @ m1 in
+    let fd0 = filter_mask_dl m0 ts0 (Fl.dlist_of_f xs0) in
+    let fd1 = filter_mask_dl m1 ts1 (Fl.dlist_of_f xs1) in
+    filter_mask_append m0 m1 ts0 ts1;
+    calc (==) {
+      filter_mask_fl m (ts0 @ ts1) (Fl.append xs0 xs1);
+    == { filter_mask_f_dl_f m _ (Fl.append xs0 xs1) }
+      Fl.flist_of_d (filter_mask_dl m (ts0 @ ts1) (Fl.dlist_of_f (Fl.append xs0 xs1)));
+    == { Fl.dlist_of_f_append xs0 xs1 }
+      Fl.flist_of_d (filter_mask_dl m (ts0 @ ts1) (Dl.append (Fl.dlist_of_f xs0) (Fl.dlist_of_f xs1)));
+    == { filter_mask_dl_append m0 m1 ts0 ts1 (Fl.dlist_of_f xs0) (Fl.dlist_of_f xs1) }
+      Fl.flist_of_d (Dl.append fd0 fd1);
+    == { Fl.dlist_of_f_append (Fl.flist_of_d fd0) (Fl.flist_of_d fd1) }
+      Fl.append (Fl.flist_of_d fd0) (Fl.flist_of_d fd1);
+    == { filter_mask_f_dl_f m0 ts0 xs0; filter_mask_f_dl_f m1 ts1 xs1 }
+      Fl.append (filter_mask_fl m0 ts0 xs0) (filter_mask_fl m1 ts1 xs1);
+    }
+
+#pop-options
