pure/Learn.Tactics.Logic.fst
@@ -8,6 +8,12 @@ open FStar.Tactics
 let iff_refl (p : Type) : squash (p <==> p)
   = ()
 
+let rew_iff_left (p0 p1 q : Type)
+    (_ : squash (p0 <==> p1))
+    (_ : squash (p1  <==> q))
+  : squash (p0 <==> q)
+  = ()
+
 let rew_iff_right (p q0 q1 : Type)
     (_ : squash (q0 <==> q1))
     (_ : squash (p  <==> q1))
@@ -16,9 +22,9 @@ let rew_iff_right (p q0 q1 : Type)
 
 let conj_morph_iff (p0 q0 p1 q1 : Type0)
     (_ : squash (p0 <==> p1))
-    (_ : squash (q0 <==> q1))
+    (eq_q : squash (p0 /\ p1) -> squash (q0 <==> q1))
   : squash ((p0 /\ q0) <==> (p1 /\ q1))
-  = ()
+  = FStar.Classical.Sugar.implies_intro _ _ eq_q
 
 let forall_morph_iff (#a : Type) (p0 p1 : a -> Type0)
       (prf : (x : a) -> squash (p0 x <==> p1 x))
@@ -32,9 +38,9 @@ let exists_morph_iff (#a : Type) (p0 p1 : a -> Type0)
 
 let impl_morph_iff (p0 q0 p1 q1 : Type0)
     (_ : squash (p0 <==> p1))
-    (_ : squash (q0 <==> q1))
+    (eq_q : squash (p0 /\ p1) -> squash (q0 <==> q1))
   : squash ((p0 ==> q0) <==> (p1 ==> q1))
-  = ()
+  = FStar.Classical.Sugar.implies_intro _ _ eq_q
 
 let iff_morph_iff (p0 q0 p1 q1 : Type0)
     (_ : squash (p0 <==> p1))
@@ -52,6 +58,17 @@ let rew_exists_unit' (p0 : U.unit' -> Type) (p1 : Type)
   : squash ((exists (u : U.unit') . p0 u) <==> p1)
   = ()
 
+let rew_forall_eq (#a : Type) (#p : a -> Type0) (x : a)
+      (h : squash (forall (x' : a) . x' =!= x ==> p x'))
+  : squash ((forall x' . p x') <==> p x)
+  = ()
+
+let rew_exists_eq (#a : Type) (#p : a -> Type0) (x : a)
+      (h : squash (forall (x' : a) . p x' ==> x' == x))
+  : squash ((exists x' . p x') <==> p x)
+  = ()
+
+
 /// Used to rewrite a [prop] to an equivalent ([<==>]) one.
 /// Solves a goal of the form [p <==> ?p']
 // TODO: currently, this can backtrack: prevent backtracking / option ?
@@ -59,11 +76,11 @@ let rec rew_iff (pre : (unit -> Tac unit) -> Tac unit) : Tac unit =
   let r () = rew_iff pre in
   first [
     (fun () -> pre r);
-    (fun () -> apply (`conj_morph_iff); iseq [r; r]);
+    (fun () -> apply (`conj_morph_iff); iseq [r; (fun () -> let _ = intro () in r ())]);
     // [rew_forall_unit'] needs to be done before [impl_morph_iff]
     (fun () -> apply (`rew_forall_unit'); r ());
     (fun () -> apply (`rew_exists_unit'); r ());
-    (fun () -> apply (`impl_morph_iff); iseq [r; r]);
+    (fun () -> apply (`impl_morph_iff); iseq [r; (fun () -> let _ = intro () in r ())]);
     (fun () -> apply (`forall_morph_iff); let _ = intro () in r ());
     (fun () -> apply (`exists_morph_iff); let _ = intro () in r ());
     (fun () -> apply (`iff_morph_iff); iseq [r; r]);
